Make verified ML-KEM available in `libcrux-ml-kem` (#329)
* Revert changes to Kyber (Round 3) for ML-KEM

* Fix swapped private key decoding

* Pull out Kyber encaps

* Make Kyber API available behind `kyber` feature

* Format

* Introduce `kyber` feature in `libcrux-kem`

* Format

* Include verified ML-KEM in `libcrux-ml-kem`

* WIP separation of verified API

* Integrating pre-verification and verified testing

* Integrating verified ML-KEM in `libcrux-kem`

* Format

* Test portable pre-verification ML-KEM 768

* fix C extraction

* Fix typo

* Give more accurate test names (`kyber...` to `mlkem...`)

* Avoid unused warning when testing

* Use `Hasher` trait to select best KDF for Kyber

* Document differences between Kyber (Round 3) and ML-KEM

* Inline ML-KEM/Kyber variant differences

* `kyber{512,768,1024}` top level modules

* Fix `kyber` feature in `libcrux-kem`

* Rename NIST KAT files for ML-KEM

* Include NIST KATs for all Kyber parameter sets

* Document single Kyber 768 KAT from boringssl

* Format

* Test Kyber on CI

* Fix insufficient feature gating

* Get rid of various warnings

* Format

* Remove commented `use` declarations

* Fix `unused_mut` warning

* Feature gating helper macros

* Fix hax extraction

* Feature flag documentation

* Fix mistaken feature guards

* Remove commented code

* `size` -> `len`

* Drop explicit dependency on `hax-lib-macros`

* Hide helper macro docs

* Formatting

* Call out the `kyber` feature more prominently

* Feature gate tests etc so `--no-std-features` tests

* cleanup; make features work

* more cleanup and docs

* update hax extraction

* fixup x64 and hax extract

* update C extraction

* update header only C code

* update C code

* install cargo hack on ci

* ci

* more updates

---------

Co-authored-by: Franziskus Kiefer <franziskuskiefer@gmail.com>

libcrux-ml-kem/src/ind_cca.rs
@@ -301,11 +301,15 @@ impl Variant for MlKem {
         shared_secret: &[u8],
         _: &MlKemCiphertext<CIPHERTEXT_SIZE>,
     ) -> [u8; 32] {
-        shared_secret.try_into().unwrap()
+        let mut out = [0u8; 32];
+        out.copy_from_slice(shared_secret);
+        out
     }
 
     #[inline(always)]
     fn entropy_preprocess<const K: usize, Hasher: Hash<K>>(randomness: &[u8]) -> [u8; 32] {
-        randomness.try_into().unwrap()
+        let mut out = [0u8; 32];
+        out.copy_from_slice(randomness);
+        out
     }
 }
