libcrux-ml-kem/src/kem/kyber/kyber512.rs
@@ -1,0 +1,158 @@
+use super::{constants::*, *};
+
+// Kyber 512 parameters
+const RANK_512: usize = 2;
+const RANKED_BYTES_PER_RING_ELEMENT_512: usize = RANK_512 * BITS_PER_RING_ELEMENT / 8;
+const T_AS_NTT_ENCODED_SIZE_512: usize =
+    (RANK_512 * COEFFICIENTS_IN_RING_ELEMENT * BITS_PER_COEFFICIENT) / 8;
+const VECTOR_U_COMPRESSION_FACTOR_512: usize = 10;
+// [hax]: hacspec/hacspec-v2#27 stealing error
+// block_len::<VECTOR_U_COMPRESSION_FACTOR_512>()
+const C1_BLOCK_SIZE_512: usize =
+    (COEFFICIENTS_IN_RING_ELEMENT * VECTOR_U_COMPRESSION_FACTOR_512) / 8;
+// [hax]: hacspec/hacspec-v2#27 stealing error
+// serialized_len::<RANK_512, C1_BLOCK_SIZE_512>()
+const C1_SIZE_512: usize = C1_BLOCK_SIZE_512 * RANK_512;
+const VECTOR_V_COMPRESSION_FACTOR_512: usize = 4;
+// [hax]: hacspec/hacspec-v2#27 stealing error
+// block_len::<VECTOR_V_COMPRESSION_FACTOR_512>()
+const C2_SIZE_512: usize = (COEFFICIENTS_IN_RING_ELEMENT * VECTOR_V_COMPRESSION_FACTOR_512) / 8;
+const CPA_PKE_SECRET_KEY_SIZE_512: usize =
+    (RANK_512 * COEFFICIENTS_IN_RING_ELEMENT * BITS_PER_COEFFICIENT) / 8;
+const CPA_PKE_PUBLIC_KEY_SIZE_512: usize = T_AS_NTT_ENCODED_SIZE_512 + 32;
+const CPA_PKE_CIPHERTEXT_SIZE_512: usize = C1_SIZE_512 + C2_SIZE_512;
+const SECRET_KEY_SIZE_512: usize =
+    CPA_PKE_SECRET_KEY_SIZE_512 + CPA_PKE_PUBLIC_KEY_SIZE_512 + H_DIGEST_SIZE + SHARED_SECRET_SIZE;
+
+const ETA1: usize = 3;
+const ETA1_RANDOMNESS_SIZE: usize = ETA1 * 64;
+const ETA2: usize = 2;
+const ETA2_RANDOMNESS_SIZE: usize = ETA2 * 64;
+
+const IMPLICIT_REJECTION_HASH_INPUT_SIZE: usize = SHARED_SECRET_SIZE + CPA_PKE_CIPHERTEXT_SIZE_512;
+
+// Kyber 512 types
+pub type MlKem512Ciphertext = MlKemCiphertext<CPA_PKE_CIPHERTEXT_SIZE_512>;
+pub type MlKem512PrivateKey = MlKemPrivateKey<SECRET_KEY_SIZE_512>;
+pub type MlKem512PublicKey = MlKemPublicKey<CPA_PKE_PUBLIC_KEY_SIZE_512>;
+
+/// Validate a public key.
+///
+/// Returns `Some(public_key)` if valid, and `None` otherwise.
+pub fn validate_public_key(public_key: MlKem512PublicKey) -> Option<MlKem512PublicKey> {
+    if super::validate_public_key::<
+        RANK_512,
+        RANKED_BYTES_PER_RING_ELEMENT_512,
+        CPA_PKE_PUBLIC_KEY_SIZE_512,
+    >(&public_key.value)
+    {
+        Some(public_key)
+    } else {
+        None
+    }
+}
+
+/// Generate ML-KEM 512 Key Pair
+pub fn generate_key_pair(
+    randomness: [u8; KEY_GENERATION_SEED_SIZE],
+) -> MlKemKeyPair<SECRET_KEY_SIZE_512, CPA_PKE_PUBLIC_KEY_SIZE_512> {
+    generate_keypair::<
+        RANK_512,
+        CPA_PKE_SECRET_KEY_SIZE_512,
+        SECRET_KEY_SIZE_512,
+        CPA_PKE_PUBLIC_KEY_SIZE_512,
+        RANKED_BYTES_PER_RING_ELEMENT_512,
+        ETA1,
+        ETA1_RANDOMNESS_SIZE,
+    >(randomness)
+}
+
+pub type MlKem512State = MlKemState<RANK_512>;
+
+pub fn generate_key_pair_unpacked(
+    randomness: [u8; KEY_GENERATION_SEED_SIZE],
+) -> (MlKem512State, MlKem512PublicKey) {
+    generate_keypair_unpacked::<
+        RANK_512,
+        CPA_PKE_SECRET_KEY_SIZE_512,
+        SECRET_KEY_SIZE_512,
+        CPA_PKE_PUBLIC_KEY_SIZE_512,
+        RANKED_BYTES_PER_RING_ELEMENT_512,
+        ETA1,
+        ETA1_RANDOMNESS_SIZE,
+    >(randomness)
+}
+
+/// Encapsulate ML-KEM 512
+pub fn encapsulate(
+    public_key: &MlKemPublicKey<CPA_PKE_PUBLIC_KEY_SIZE_512>,
+    randomness: [u8; SHARED_SECRET_SIZE],
+) -> (
+    MlKemCiphertext<CPA_PKE_CIPHERTEXT_SIZE_512>,
+    MlKemSharedSecret,
+) {
+    super::encapsulate::<
+        RANK_512,
+        CPA_PKE_CIPHERTEXT_SIZE_512,
+        CPA_PKE_PUBLIC_KEY_SIZE_512,
+        T_AS_NTT_ENCODED_SIZE_512,
+        C1_SIZE_512,
+        C2_SIZE_512,
+        VECTOR_U_COMPRESSION_FACTOR_512,
+        VECTOR_V_COMPRESSION_FACTOR_512,
+        C1_BLOCK_SIZE_512,
+        ETA1,
+        ETA1_RANDOMNESS_SIZE,
+        ETA2,
+        ETA2_RANDOMNESS_SIZE,
+    >(public_key, randomness)
+}
+
+/// Decapsulate ML-KEM 512
+pub fn decapsulate(
+    secret_key: &MlKemPrivateKey<SECRET_KEY_SIZE_512>,
+    ciphertext: &MlKemCiphertext<CPA_PKE_CIPHERTEXT_SIZE_512>,
+) -> [u8; SHARED_SECRET_SIZE] {
+    super::decapsulate::<
+        RANK_512,
+        SECRET_KEY_SIZE_512,
+        CPA_PKE_SECRET_KEY_SIZE_512,
+        CPA_PKE_PUBLIC_KEY_SIZE_512,
+        CPA_PKE_CIPHERTEXT_SIZE_512,
+        T_AS_NTT_ENCODED_SIZE_512,
+        C1_SIZE_512,
+        C2_SIZE_512,
+        VECTOR_U_COMPRESSION_FACTOR_512,
+        VECTOR_V_COMPRESSION_FACTOR_512,
+        C1_BLOCK_SIZE_512,
+        ETA1,
+        ETA1_RANDOMNESS_SIZE,
+        ETA2,
+        ETA2_RANDOMNESS_SIZE,
+        IMPLICIT_REJECTION_HASH_INPUT_SIZE,
+    >(secret_key, ciphertext)
+}
+
+pub fn decapsulate_unpacked(
+    state: &MlKem512State,
+    ciphertext: &MlKemCiphertext<CPA_PKE_CIPHERTEXT_SIZE_512>,
+) -> [u8; SHARED_SECRET_SIZE] {
+    super::decapsulate_unpacked::<
+        RANK_512,
+        SECRET_KEY_SIZE_512,
+        CPA_PKE_SECRET_KEY_SIZE_512,
+        CPA_PKE_PUBLIC_KEY_SIZE_512,
+        CPA_PKE_CIPHERTEXT_SIZE_512,
+        T_AS_NTT_ENCODED_SIZE_512,
+        C1_SIZE_512,
+        C2_SIZE_512,
+        VECTOR_U_COMPRESSION_FACTOR_512,
+        VECTOR_V_COMPRESSION_FACTOR_512,
+        C1_BLOCK_SIZE_512,
+        ETA1,
+        ETA1_RANDOMNESS_SIZE,
+        ETA2,
+        ETA2_RANDOMNESS_SIZE,
+        IMPLICIT_REJECTION_HASH_INPUT_SIZE,
+    >(state, ciphertext)
+}
