libcrux-ml-kem/src/kem/kyber/matrix.rs
@@ -1,0 +1,158 @@
+use super::{
+    arithmetic::{
+        add_to_ring_element, barrett_reduce, montgomery_reduce, to_standard_domain,
+        PolynomialRingElement,
+    },
+    constants::COEFFICIENTS_IN_RING_ELEMENT,
+    helper::cloop,
+    ntt::{invert_ntt_montgomery, ntt_multiply},
+    sampling::sample_from_xof,
+};
+
+#[inline(always)]
+#[allow(non_snake_case)]
+pub(in crate::kem::kyber) fn sample_matrix_A<const K: usize>(
+    seed: [u8; 34],
+    transpose: bool,
+) -> [[PolynomialRingElement; K]; K] {
+    let mut A_transpose = [[PolynomialRingElement::ZERO; K]; K];
+
+    for i in 0..K {
+        let mut seeds = [seed; K];
+        for j in 0..K {
+            seeds[j][32] = i as u8;
+            seeds[j][33] = j as u8;
+        }
+        let sampled = sample_from_xof(seeds);
+        for j in 0..K {
+            // A[i][j] = A_transpose[j][i]
+            if transpose {
+                A_transpose[j][i] = sampled[j];
+            } else {
+                A_transpose[i][j] = sampled[j];
+            }
+        }
+    }
+
+    A_transpose
+}
+
+/// The following functions compute various expressions involving
+/// vectors and matrices. The computation of these expressions has been
+/// abstracted away into these functions in order to save on loop iterations.
+
+/// Compute v − InverseNTT(sᵀ ◦ NTT(u))
+#[inline(always)]
+pub(in crate::kem::kyber) fn compute_message<const K: usize>(
+    v: &PolynomialRingElement,
+    secret_as_ntt: &[PolynomialRingElement; K],
+    u_as_ntt: &[PolynomialRingElement; K],
+) -> PolynomialRingElement {
+    let mut result = PolynomialRingElement::ZERO;
+
+    for i in 0..K {
+        let product = ntt_multiply(&secret_as_ntt[i], &u_as_ntt[i]);
+        result = add_to_ring_element::<K>(result, &product);
+    }
+
+    result = invert_ntt_montgomery::<K>(result);
+
+    for i in 0..COEFFICIENTS_IN_RING_ELEMENT {
+        let coefficient_normal_form = montgomery_reduce(result.coefficients[i] * 1441);
+        result.coefficients[i] = barrett_reduce(v.coefficients[i] - coefficient_normal_form);
+    }
+
+    result
+}
+
+/// Compute InverseNTT(tᵀ ◦ r̂) + e₂ + message
+#[inline(always)]
+pub(in crate::kem::kyber) fn compute_ring_element_v<const K: usize>(
+    t_as_ntt: &[PolynomialRingElement; K],
+    r_as_ntt: &[PolynomialRingElement; K],
+    error_2: &PolynomialRingElement,
+    message: &PolynomialRingElement,
+) -> PolynomialRingElement {
+    let mut result = PolynomialRingElement::ZERO;
+
+    for i in 0..K {
+        let product = ntt_multiply(&t_as_ntt[i], &r_as_ntt[i]);
+        result = add_to_ring_element::<K>(result, &product);
+    }
+
+    result = invert_ntt_montgomery::<K>(result);
+
+    for i in 0..COEFFICIENTS_IN_RING_ELEMENT {
+        let coefficient_normal_form = montgomery_reduce(result.coefficients[i] * 1441);
+        result.coefficients[i] = barrett_reduce(
+            coefficient_normal_form + error_2.coefficients[i] + message.coefficients[i],
+        );
+    }
+
+    result
+}
+
+/// Compute u := InvertNTT(Aᵀ ◦ r̂) + e₁
+#[inline(always)]
+pub(in crate::kem::kyber) fn compute_vector_u<const K: usize>(
+    a_as_ntt: &[[PolynomialRingElement; K]; K],
+    r_as_ntt: &[PolynomialRingElement; K],
+    error_1: &[PolynomialRingElement; K],
+) -> [PolynomialRingElement; K] {
+    let mut result = [PolynomialRingElement::ZERO; K];
+
+    cloop! {
+        for (i, row) in a_as_ntt.iter().enumerate() {
+            cloop! {
+                for (j, a_element) in row.iter().enumerate() {
+                    let product = ntt_multiply(a_element, &r_as_ntt[j]);
+                    result[i] = add_to_ring_element::<K>(result[i], &product);
+                }
+            }
+
+            result[i] = invert_ntt_montgomery::<K>(result[i]);
+
+            for j in 0..COEFFICIENTS_IN_RING_ELEMENT {
+                let coefficient_normal_form = montgomery_reduce(result[i].coefficients[j] * 1441);
+
+                result[i].coefficients[j] =
+                    barrett_reduce(coefficient_normal_form + error_1[i].coefficients[j]);
+            }
+        }
+    }
+
+    result
+}
+
+/// Compute Â ◦ ŝ + ê
+#[inline(always)]
+#[allow(non_snake_case)]
+pub(in crate::kem::kyber) fn compute_As_plus_e<const K: usize>(
+    matrix_A: &[[PolynomialRingElement; K]; K],
+    s_as_ntt: &[PolynomialRingElement; K],
+    error_as_ntt: &[PolynomialRingElement; K],
+) -> [PolynomialRingElement; K] {
+    let mut result = [PolynomialRingElement::ZERO; K];
+
+    cloop! {
+        for (i, row) in matrix_A.iter().enumerate() {
+            cloop! {
+                for (j, matrix_element) in row.iter().enumerate() {
+                    let product = ntt_multiply(matrix_element, &s_as_ntt[j]);
+                    result[i] = add_to_ring_element::<K>(result[i], &product);
+                }
+            }
+
+            for j in 0..COEFFICIENTS_IN_RING_ELEMENT {
+                // The coefficients are of the form aR^{-1} mod q, which means
+                // calling to_montgomery_domain() on them should return a mod q.
+                let coefficient_normal_form = to_standard_domain(result[i].coefficients[j]);
+
+                result[i].coefficients[j] =
+                    barrett_reduce(coefficient_normal_form + error_as_ntt[i].coefficients[j])
+            }
+        }
+    }
+
+    result
+}
