libcrux-ml-kem/proofs/fstar/extraction/Libcrux_ml_kem.Types.fsti
@@ -3,11 +3,23 @@ module Libcrux_ml_kem.Types
 open Core
 open FStar.Mul
 
+/// The number of bytes
+val impl_6__len: v_SIZE: usize -> Prims.unit
+  -> Prims.Pure usize Prims.l_True (fun _ -> Prims.l_True)
+
+/// The number of bytes
+val impl_12__len: v_SIZE: usize -> Prims.unit
+  -> Prims.Pure usize Prims.l_True (fun _ -> Prims.l_True)
+
+/// The number of bytes
+val impl_18__len: v_SIZE: usize -> Prims.unit
+  -> Prims.Pure usize Prims.l_True (fun _ -> Prims.l_True)
+
 ///An ML-KEM Ciphertext
 type t_MlKemCiphertext (v_SIZE: usize) = { f_value:t_Array u8 v_SIZE }
 
 [@@ FStar.Tactics.Typeclasses.tcinstance]
-let impl_1 (v_SIZE: usize) : Core.Convert.t_AsRef (t_MlKemCiphertext v_SIZE) (t_Slice u8) =
+let impl_1 (v_SIZE: usize) : Core.Convert.t_AsRef #(t_MlKemCiphertext v_SIZE) #(t_Slice u8) =
   {
     f_as_ref_pre = (fun (self: t_MlKemCiphertext v_SIZE) -> true);
     f_as_ref_post = (fun (self: t_MlKemCiphertext v_SIZE) (out: t_Slice u8) -> true);
@@ -15,7 +27,7 @@ let impl_1 (v_SIZE: usize) : Core.Convert.t_AsRef (t_MlKemCiphertext v_SIZE) (t_
   }
 
 [@@ FStar.Tactics.Typeclasses.tcinstance]
-let impl_2 (v_SIZE: usize) : Core.Convert.t_From (t_MlKemCiphertext v_SIZE) (t_Array u8 v_SIZE) =
+let impl_2 (v_SIZE: usize) : Core.Convert.t_From #(t_MlKemCiphertext v_SIZE) #(t_Array u8 v_SIZE) =
   {
     f_from_pre = (fun (value: t_Array u8 v_SIZE) -> true);
     f_from_post = (fun (value: t_Array u8 v_SIZE) (out: t_MlKemCiphertext v_SIZE) -> true);
@@ -23,7 +35,7 @@ let impl_2 (v_SIZE: usize) : Core.Convert.t_From (t_MlKemCiphertext v_SIZE) (t_A
   }
 
 [@@ FStar.Tactics.Typeclasses.tcinstance]
-let impl_3 (v_SIZE: usize) : Core.Convert.t_From (t_MlKemCiphertext v_SIZE) (t_Array u8 v_SIZE) =
+let impl_3 (v_SIZE: usize) : Core.Convert.t_From #(t_MlKemCiphertext v_SIZE) #(t_Array u8 v_SIZE) =
   {
     f_from_pre = (fun (value: t_Array u8 v_SIZE) -> true);
     f_from_post = (fun (value: t_Array u8 v_SIZE) (out: t_MlKemCiphertext v_SIZE) -> true);
@@ -34,7 +46,7 @@ let impl_3 (v_SIZE: usize) : Core.Convert.t_From (t_MlKemCiphertext v_SIZE) (t_A
   }
 
 [@@ FStar.Tactics.Typeclasses.tcinstance]
-let impl_4 (v_SIZE: usize) : Core.Convert.t_From (t_Array u8 v_SIZE) (t_MlKemCiphertext v_SIZE) =
+let impl_4 (v_SIZE: usize) : Core.Convert.t_From #(t_Array u8 v_SIZE) #(t_MlKemCiphertext v_SIZE) =
   {
     f_from_pre = (fun (value: t_MlKemCiphertext v_SIZE) -> true);
     f_from_post = (fun (value: t_MlKemCiphertext v_SIZE) (out: t_Array u8 v_SIZE) -> true);
@@ -49,7 +61,7 @@ val impl_6__as_slice (v_SIZE: usize) (self: t_MlKemCiphertext v_SIZE)
 type t_MlKemPrivateKey (v_SIZE: usize) = { f_value:t_Array u8 v_SIZE }
 
 [@@ FStar.Tactics.Typeclasses.tcinstance]
-let impl_7 (v_SIZE: usize) : Core.Convert.t_AsRef (t_MlKemPrivateKey v_SIZE) (t_Slice u8) =
+let impl_7 (v_SIZE: usize) : Core.Convert.t_AsRef #(t_MlKemPrivateKey v_SIZE) #(t_Slice u8) =
   {
     f_as_ref_pre = (fun (self: t_MlKemPrivateKey v_SIZE) -> true);
     f_as_ref_post = (fun (self: t_MlKemPrivateKey v_SIZE) (out: t_Slice u8) -> true);
@@ -57,7 +69,7 @@ let impl_7 (v_SIZE: usize) : Core.Convert.t_AsRef (t_MlKemPrivateKey v_SIZE) (t_
   }
 
 [@@ FStar.Tactics.Typeclasses.tcinstance]
-let impl_8 (v_SIZE: usize) : Core.Convert.t_From (t_MlKemPrivateKey v_SIZE) (t_Array u8 v_SIZE) =
+let impl_8 (v_SIZE: usize) : Core.Convert.t_From #(t_MlKemPrivateKey v_SIZE) #(t_Array u8 v_SIZE) =
   {
     f_from_pre = (fun (value: t_Array u8 v_SIZE) -> true);
     f_from_post = (fun (value: t_Array u8 v_SIZE) (out: t_MlKemPrivateKey v_SIZE) -> true);
@@ -65,7 +77,7 @@ let impl_8 (v_SIZE: usize) : Core.Convert.t_From (t_MlKemPrivateKey v_SIZE) (t_A
   }
 
 [@@ FStar.Tactics.Typeclasses.tcinstance]
-let impl_9 (v_SIZE: usize) : Core.Convert.t_From (t_MlKemPrivateKey v_SIZE) (t_Array u8 v_SIZE) =
+let impl_9 (v_SIZE: usize) : Core.Convert.t_From #(t_MlKemPrivateKey v_SIZE) #(t_Array u8 v_SIZE) =
   {
     f_from_pre = (fun (value: t_Array u8 v_SIZE) -> true);
     f_from_post = (fun (value: t_Array u8 v_SIZE) (out: t_MlKemPrivateKey v_SIZE) -> true);
@@ -76,7 +88,7 @@ let impl_9 (v_SIZE: usize) : Core.Convert.t_From (t_MlKemPrivateKey v_SIZE) (t_A
   }
 
 [@@ FStar.Tactics.Typeclasses.tcinstance]
-let impl_10 (v_SIZE: usize) : Core.Convert.t_From (t_Array u8 v_SIZE) (t_MlKemPrivateKey v_SIZE) =
+let impl_10 (v_SIZE: usize) : Core.Convert.t_From #(t_Array u8 v_SIZE) #(t_MlKemPrivateKey v_SIZE) =
   {
     f_from_pre = (fun (value: t_MlKemPrivateKey v_SIZE) -> true);
     f_from_post = (fun (value: t_MlKemPrivateKey v_SIZE) (out: t_Array u8 v_SIZE) -> true);
@@ -91,7 +103,7 @@ val impl_12__as_slice (v_SIZE: usize) (self: t_MlKemPrivateKey v_SIZE)
 type t_MlKemPublicKey (v_SIZE: usize) = { f_value:t_Array u8 v_SIZE }
 
 [@@ FStar.Tactics.Typeclasses.tcinstance]
-let impl_13 (v_SIZE: usize) : Core.Convert.t_AsRef (t_MlKemPublicKey v_SIZE) (t_Slice u8) =
+let impl_13 (v_SIZE: usize) : Core.Convert.t_AsRef #(t_MlKemPublicKey v_SIZE) #(t_Slice u8) =
   {
     f_as_ref_pre = (fun (self: t_MlKemPublicKey v_SIZE) -> true);
     f_as_ref_post = (fun (self: t_MlKemPublicKey v_SIZE) (out: t_Slice u8) -> true);
@@ -99,7 +111,7 @@ let impl_13 (v_SIZE: usize) : Core.Convert.t_AsRef (t_MlKemPublicKey v_SIZE) (t_
   }
 
 [@@ FStar.Tactics.Typeclasses.tcinstance]
-let impl_14 (v_SIZE: usize) : Core.Convert.t_From (t_MlKemPublicKey v_SIZE) (t_Array u8 v_SIZE) =
+let impl_14 (v_SIZE: usize) : Core.Convert.t_From #(t_MlKemPublicKey v_SIZE) #(t_Array u8 v_SIZE) =
   {
     f_from_pre = (fun (value: t_Array u8 v_SIZE) -> true);
     f_from_post = (fun (value: t_Array u8 v_SIZE) (out: t_MlKemPublicKey v_SIZE) -> true);
@@ -107,7 +119,7 @@ let impl_14 (v_SIZE: usize) : Core.Convert.t_From (t_MlKemPublicKey v_SIZE) (t_A
   }
 
 [@@ FStar.Tactics.Typeclasses.tcinstance]
-let impl_15 (v_SIZE: usize) : Core.Convert.t_From (t_MlKemPublicKey v_SIZE) (t_Array u8 v_SIZE) =
+let impl_15 (v_SIZE: usize) : Core.Convert.t_From #(t_MlKemPublicKey v_SIZE) #(t_Array u8 v_SIZE) =
   {
     f_from_pre = (fun (value: t_Array u8 v_SIZE) -> true);
     f_from_post = (fun (value: t_Array u8 v_SIZE) (out: t_MlKemPublicKey v_SIZE) -> true);
@@ -118,7 +130,7 @@ let impl_15 (v_SIZE: usize) : Core.Convert.t_From (t_MlKemPublicKey v_SIZE) (t_A
   }
 
 [@@ FStar.Tactics.Typeclasses.tcinstance]
-let impl_16 (v_SIZE: usize) : Core.Convert.t_From (t_Array u8 v_SIZE) (t_MlKemPublicKey v_SIZE) =
+let impl_16 (v_SIZE: usize) : Core.Convert.t_From #(t_Array u8 v_SIZE) #(t_MlKemPublicKey v_SIZE) =
   {
     f_from_pre = (fun (value: t_MlKemPublicKey v_SIZE) -> true);
     f_from_post = (fun (value: t_MlKemPublicKey v_SIZE) (out: t_Array u8 v_SIZE) -> true);
@@ -130,7 +142,7 @@ val impl_18__as_slice (v_SIZE: usize) (self: t_MlKemPublicKey v_SIZE)
     : Prims.Pure (t_Array u8 v_SIZE) Prims.l_True (fun _ -> Prims.l_True)
 
 [@@ FStar.Tactics.Typeclasses.tcinstance]
-let impl_5 (v_SIZE: usize) : Core.Convert.t_TryFrom (t_MlKemCiphertext v_SIZE) (t_Slice u8) =
+let impl_5 (v_SIZE: usize) : Core.Convert.t_TryFrom #(t_MlKemCiphertext v_SIZE) #(t_Slice u8) =
   {
     f_Error = Core.Array.t_TryFromSliceError;
     f_try_from_pre = (fun (value: t_Slice u8) -> true);
@@ -156,7 +168,7 @@ let impl_5 (v_SIZE: usize) : Core.Convert.t_TryFrom (t_MlKemCiphertext v_SIZE) (
   }
 
 [@@ FStar.Tactics.Typeclasses.tcinstance]
-let impl_11 (v_SIZE: usize) : Core.Convert.t_TryFrom (t_MlKemPrivateKey v_SIZE) (t_Slice u8) =
+let impl_11 (v_SIZE: usize) : Core.Convert.t_TryFrom #(t_MlKemPrivateKey v_SIZE) #(t_Slice u8) =
   {
     f_Error = Core.Array.t_TryFromSliceError;
     f_try_from_pre = (fun (value: t_Slice u8) -> true);
@@ -182,7 +194,7 @@ let impl_11 (v_SIZE: usize) : Core.Convert.t_TryFrom (t_MlKemPrivateKey v_SIZE) 
   }
 
 [@@ FStar.Tactics.Typeclasses.tcinstance]
-let impl_17 (v_SIZE: usize) : Core.Convert.t_TryFrom (t_MlKemPublicKey v_SIZE) (t_Slice u8) =
+let impl_17 (v_SIZE: usize) : Core.Convert.t_TryFrom #(t_MlKemPublicKey v_SIZE) #(t_Slice u8) =
   {
     f_Error = Core.Array.t_TryFromSliceError;
     f_try_from_pre = (fun (value: t_Slice u8) -> true);
@@ -219,6 +231,14 @@ val impl__from
       (sk: t_MlKemPrivateKey v_PRIVATE_KEY_SIZE)
       (pk: t_MlKemPublicKey v_PUBLIC_KEY_SIZE)
     : Prims.Pure (t_MlKemKeyPair v_PRIVATE_KEY_SIZE v_PUBLIC_KEY_SIZE)
+      Prims.l_True
+      (fun _ -> Prims.l_True)
+
+/// Separate this key into the public and private key.
+val impl__into_parts
+      (v_PRIVATE_KEY_SIZE v_PUBLIC_KEY_SIZE: usize)
+      (self: t_MlKemKeyPair v_PRIVATE_KEY_SIZE v_PUBLIC_KEY_SIZE)
+    : Prims.Pure (t_MlKemPrivateKey v_PRIVATE_KEY_SIZE & t_MlKemPublicKey v_PUBLIC_KEY_SIZE)
       Prims.l_True
       (fun _ -> Prims.l_True)
 
