libcrux-ml-kem/proofs/fstar/extraction/Libcrux_ml_kem.Vector.Avx2.Serialize.fsti
@@ -9,9 +9,6 @@ val deserialize_1_ (bytes: t_Slice u8)
 val deserialize_10_ (bytes: t_Slice u8)
     : Prims.Pure Core.Core_arch.X86.t____m256i Prims.l_True (fun _ -> Prims.l_True)
 
-val deserialize_11_ (bytes: t_Slice u8)
-    : Prims.Pure Core.Core_arch.X86.t____m256i Prims.l_True (fun _ -> Prims.l_True)
-
 val deserialize_12_ (bytes: t_Slice u8)
     : Prims.Pure Core.Core_arch.X86.t____m256i Prims.l_True (fun _ -> Prims.l_True)
 
@@ -27,14 +24,17 @@ val serialize_1_ (vector: Core.Core_arch.X86.t____m256i)
 val serialize_10_ (vector: Core.Core_arch.X86.t____m256i)
     : Prims.Pure (t_Array u8 (sz 20)) Prims.l_True (fun _ -> Prims.l_True)
 
-val serialize_11_ (vector: Core.Core_arch.X86.t____m256i)
-    : Prims.Pure (t_Array u8 (sz 22)) Prims.l_True (fun _ -> Prims.l_True)
-
 val serialize_12_ (vector: Core.Core_arch.X86.t____m256i)
     : Prims.Pure (t_Array u8 (sz 24)) Prims.l_True (fun _ -> Prims.l_True)
+
+val serialize_5_ (vector: Core.Core_arch.X86.t____m256i)
+    : Prims.Pure (t_Array u8 (sz 10)) Prims.l_True (fun _ -> Prims.l_True)
 
 val serialize_4_ (vector: Core.Core_arch.X86.t____m256i)
     : Prims.Pure (t_Array u8 (sz 8)) Prims.l_True (fun _ -> Prims.l_True)
 
-val serialize_5_ (vector: Core.Core_arch.X86.t____m256i)
-    : Prims.Pure (t_Array u8 (sz 10)) Prims.l_True (fun _ -> Prims.l_True)
+val deserialize_11_ (bytes: t_Slice u8)
+    : Prims.Pure Core.Core_arch.X86.t____m256i Prims.l_True (fun _ -> Prims.l_True)
+
+val serialize_11_ (vector: Core.Core_arch.X86.t____m256i)
+    : Prims.Pure (t_Array u8 (sz 22)) Prims.l_True (fun _ -> Prims.l_True)
