libcrux-ml-kem/proofs/fstar/extraction/Libcrux_ml_kem.Vector.Traits.fsti
@@ -3,7 +3,7 @@ module Libcrux_ml_kem.Vector.Traits
 open Core
 open FStar.Mul
 
-class t_Operations (v_Self: Type0) = {
+class t_Operations (#v_Self: Type0) = {
   [@@@ FStar.Tactics.Typeclasses.no_method]_super_11581440318597584651:Core.Marker.t_Copy v_Self;
   [@@@ FStar.Tactics.Typeclasses.no_method]_super_9442900250278684536:Core.Clone.t_Clone v_Self;
   f_ZERO_pre:Prims.unit -> bool;
@@ -181,13 +181,13 @@ class t_Operations (v_Self: Type0) = {
         (fun result -> f_rej_sample_post x0 x1 result)
 }
 
-let v_FIELD_ELEMENTS_IN_VECTOR: usize = Rust_primitives.Hax.dropped_body
+let v_FIELD_ELEMENTS_IN_VECTOR: usize = sz 16
 
-let v_FIELD_MODULUS: i16 = Rust_primitives.Hax.dropped_body
+let v_FIELD_MODULUS: i16 = 3329s
 
-let v_INVERSE_OF_MODULUS_MOD_MONTGOMERY_R: u32 = Rust_primitives.Hax.dropped_body
+let v_INVERSE_OF_MODULUS_MOD_MONTGOMERY_R: u32 = 62209ul
 
-let v_MONTGOMERY_R_SQUARED_MOD_FIELD_MODULUS: i16 = Rust_primitives.Hax.dropped_body
+let v_MONTGOMERY_R_SQUARED_MOD_FIELD_MODULUS: i16 = 1353s
 
 val decompress_1_ (#v_T: Type0) {| i1: t_Operations v_T |} (v: v_T)
     : Prims.Pure v_T Prims.l_True (fun _ -> Prims.l_True)
